It worksgit add main.S (WIP)

argsParseProgScript.sml
@@ -1,12 +1,9 @@
-open preamble ml_progLib ml_translatorLib
-     basisFunctionsLib fsioProgLib
-     cfTacticsLib cfLetAutoLib fsioConstantsProgTheory
-
+open preamble basis compilationLib
 open argsParseTheory pegTheory pegexecTheory
 
 val _ = new_theory"argsParseProg";
 
-val _ = translation_extends"fsioProg";
+val _ = translation_extends"basisProg";
 
 
 val INTRO_FLOOKUP = Q.store_thm("INTRO_FLOOKUP",
@@ -70,14 +67,79 @@ val parse_args_side = Q.prove(
      fs [definition"destresult_side_def"])) |> update_precondition;
 
 val print_args_def = Define`
-  print_args args =
+print_args args =
     let prntarg a = case a of
-                      | Option x (SOME y) => strlit (x ++ " -> " ++ y)
-                      | Option x NONE => strlit (x ++ " -> NONE")
-                      | Single x => strlit x
-    in case parse_args args of
-         | NONE   => (strlit "Error")
-         | SOME l => concatWith (strlit "\n") (MAP prntarg l)
+                      | Option x (SOME y) => implode (x ++ " -> " ++ y)
+                      | Option x NONE => implode (x ++ " -> NONE")
+                      | Single x => implode x;
+        argstr = explode (concatWith (implode " ") args)
+    in case parse_args argstr of
+         | NONE   => (implode "Error")
+         | SOME l => concatWith (implode "\n") (MAP prntarg l)
 `;
+
+val r = translate print_args_def;
+
+val main = process_topdecs
+  `fun main u =
+     let
+       val cl = Commandline.arguments ()
+       val args = print_args cl
+       val ok = TextIO.print_string args
+     in TextIO.print_newline() end`;
+
+val () = append_prog main;
+
+val st = get_ml_prog_state();
+
+val main_spec = Q.store_thm("main",
+  `!fs ls b bv.
+   app (p:'ffi ffi_proj) ^(fetch_v "main" st) [Conv NONE []]
+   (STDIO fs * COMMANDLINE cl)
+   (POSTv uv. &UNIT_TYPE () uv *
+      (STDIO (add_stdout fs (explode (print_args (MAP implode (TL cl))) ++ "\n"))) *
+      COMMANDLINE cl)`,
+  xcf "main" st \\
+  cases_on`¬ STD_streams fs` >-(fs[STDIO_def] >> xpull) >>
+  xlet_auto >- (xcon \\ xsimpl) \\
+  reverse(Cases_on`wfcl cl`) >- (fs[COMMANDLINE_def] \\ xpull) \\
+  `¬NULL cl` by fs[wfcl_def] \\
+  xlet_auto >- xsimpl \\
+  xlet_auto >- xsimpl \\
+  xlet`POSTv uv.  &UNIT_TYPE () uv * COMMANDLINE cl *
+        STDIO (add_stdout fs (explode (print_args (MAP implode (TL cl)))))`
+  >- (xapp >> xsimpl >> instantiate >> xsimpl >>
+      (* TODO: why? *)
+      qexists_tac`COMMANDLINE cl` >> xsimpl >>
+      qexists_tac`fs` >> rw [MAP_TL] >> xsimpl) >>
+  xlet_auto >- (xcon >> xsimpl) >>
+  xapp >> xsimpl >>
+  qmatch_goalsub_abbrev_tac`STDIO fs'` \\
+  CONV_TAC SWAP_EXISTS_CONV \\ qexists_tac`fs'` \\
+  unabbrev_all_tac \\
+  simp[concatWith_CONCAT_WITH,MAP_TL,implode_def] \\
+  xsimpl >> fs[] >>
+  imp_res_tac STD_streams_stdout >>
+  imp_res_tac add_stdo_o >> xsimpl);
+
+val st = get_ml_prog_state();
+
+val spec = main_spec |> SPEC_ALL |> UNDISCH_ALL |>
+            SIMP_RULE(srw_ss())[STDIO_def] |>
+            add_basis_proj;
+
+val name = "main";
+val (call_thm_main, main_prog_tm) = call_thm st name spec;
+val main_prog_def = Define`main_prog = ^main_prog_tm`;
+
+val main_semantics = save_thm("main_semantics",
+  call_thm_main
+  |> ONCE_REWRITE_RULE[GSYM main_prog_def]
+  |> DISCH_ALL
+  |> SIMP_RULE std_ss [LENGTH,APPEND,AND_IMP_INTRO,STD_streams_add_stdout,GSYM CONJ_ASSOC]);
+
+val main_compiled = save_thm("main_compiled",
+  compile_x64 500 500 "main" main_prog_def);
+
 
 val _ = export_theory()
